\begin{proposicion}\label{sist-impl}
                Sean $c_1,\ldots,c_m$ en $\K$. Si $(x_1,\ldots,x_n) \in \K^n$  es solución del sistema de ecuaciones
                \begin{equation*}
                \begin{matrix}
                a_{11}x_1& + &a_{12}x_2& + &\cdots& + &a_{1n}x_n &= &y_1\\
                \vdots&  &\vdots& &&  &\vdots \\
                a_{m1}x_1& + &a_{m2}x_2& + &\cdots& + &a_{mn}x_n &=&y_m.
                \end{matrix}
                \end{equation*}
                 entonces $(x_1,\ldots,x_n)$ también es solución de la ecuación
                 \begin{equation*}
                 \left(\sum_{i=1}^{m}c_{i}a_{i1}\right)x_1 + \cdots +  	\left(\sum_{i=1}^{m}c_{i}a_{in}\right)x_n = \sum_{i=1}^{m}	c_{i}y_{i},
                 \end{equation*}
            \end{proposicion}